Some cleanup in L6_to_Clight and in timing instances. Will refactor the timing instances now, add the script to run tests with timing, and then this will be ready to merge into master

plugin/certicoq.ml
@@ -9,6 +9,7 @@ open Term_quoter
 open ExceptionMonad   
 open AstCommon
 
+
 let pr_char c = str (Char.escaped c)
    
 let pr_char_list =
@@ -18,7 +19,28 @@ let rec coq_nat_of_int x =
   match x with
   | 0 -> Datatypes.O
   | n -> Datatypes.S (coq_nat_of_int (pred n))
-   
+
+
+let pcuic_size' a p =
+  match p with
+  | Coq_tRel n -> a+1
+  | Coq_tMeta n -> a+1
+  | Coq_tVar id -> a+1
+  | Coq_tEvar -> a+1 
+  | Coq_tSort -> a+1
+  | Coq_tProd n t1 t2 ->  pcuic_size (pcuic_size (a+1) t1) t2
+| Coq_tLambda n t b -> pcuic_size (a+1) 1 
+| Coq_tLetIn n t1 ty t2 -> pcuic_size (pcuic_size (a+1) t1) t2 
+| Coq_tApp t1 t2 ->  of term * term
+| Coq_tConst of kername * universe_instance
+| Coq_tInd of inductive * universe_instance
+| Coq_tConstruct of inductive * nat * universe_instance
+| Coq_tCase of (inductive * nat) * term * term * (nat * term) list
+| Coq_tProj of projection * term
+| Coq_tFix of term mfixpoint * nat
+| Coq_tCoFix of term mfixpoint * nat
+| _ -> "unimplemented"
+                     
 let compile gr =
   let env = Global.env () in
   let sigma = Evd.from_env env in
@@ -36,9 +58,12 @@ let compile gr =
   match AllInstances.compile_template_L7 fuel term with
   | Ret ((nenv, header), prg) ->
      Feedback.msg_debug (str"Finished compiling, printing to file.");
-     let str = quote_string (Names.KerName.to_string (Names.Constant.canonical const) ^ ".c") in
+     let time = Unix.gettimeofday() in
+     let cstr = quote_string (Names.KerName.to_string (Names.Constant.canonical const) ^ ".c") in
      let hstr = quote_string (Names.KerName.to_string (Names.Constant.canonical const) ^ ".h") in
-     AllInstances.printProg (nenv,prg) str;
-     AllInstances.printProg (nenv,header) hstr
+     AllInstances.printProg (nenv,prg) cstr;
+     AllInstances.printProg (nenv,header) hstr;
+     let time = (Unix.gettimeofday() -. time) in
+     Feedback.msg_debug (str(Printf.sprintf "Printed to file in %f s.." time))
   | Exc s ->
      CErrors.user_err ~hdr:"template-coq" (str "Could not compile: " ++ pr_char_list s)
