theories/L1g/instances.v
@@ -79,9 +79,10 @@ Local Generalizable Variable Lj.
 
 Definition translateTo `{F:utils.Fuel} `{CerticoqTranslation (Program L1g.compile.Term) Lj}
            (p:Template.Ast.program): exception Lj :=
-  (AstCommon.timePhase "L1 to L2")
-    (fun (_:Datatypes.unit) => (let l1g:= L1g.compile.program_Program p in
-     translate (Program L1g.compile.Term) Lj l1g)).
+  let l1g := ((AstCommon.timePhase "L1 to L2")
+                (fun (_:Datatypes.unit) =>
+                   L1g.compile.program_Program p)) in 
+     translate (Program L1g.compile.Term) Lj l1g.
 
 Arguments translateTo {F} Lj {H} p.
 
